## Тест на простой сетке из двух областей

|y\x|  1  |  2  |  3   
|:-:| :-: | :-: | :-:
| 1 |  4  |  5  |  6  
| 2 |  1  |  2  |  3



---

$$-\frac{1}{r}\frac{\partial}{\partial r}(r\lambda \frac{\partial u}{\partial r}) - \frac{1}{r^2}\frac{\partial}{\partial \phi}(\lambda \frac{\partial u}{\partial \phi}) + \gamma u = f$$

Пусть $u(r,\phi) = r$, тогда

$$-\frac{1}{r}\frac{\partial}{\partial r}(r\lambda ) + \gamma r = f$$

Пусть $\lambda = r, \gamma = 1$, тогда

$$-2 + r = f \Rightarrow f = r - 2$$

---

$$
-\frac{1}{r}\frac{\partial}{\partial r}(r\lambda \frac{\partial u}{\partial r}) - \frac{1}{r^2}\frac{\partial}{\partial \phi}(\lambda \frac{\partial u}{\partial \phi}) + \gamma u = f
$$

Пусть $u(r, \phi) = r$, тогда

$$
-\frac{1}{r}\frac{\partial}{\partial r}(r\lambda ) + \gamma r = f
$$

Пусть $\lambda = 1, \gamma = 1$, тогда

$$
-\frac{1}{r} + r = f \\
f = r - \frac{1}{r}
$$

---

$$
  -\frac{1}{r}\frac{\partial}{\partial r}(r\lambda \frac{\partial u}{\partial r}) - \frac{1}{r^2}\frac{\partial}{\partial \phi}(\lambda \frac{\partial u}{\partial \phi}) + \gamma u = f
$$

Пусть $u(r, \phi) = \phi$, тогда

$$
  - \frac{1}{r^2}\frac{\partial}{\partial \phi}(\lambda ) + \gamma \phi = f
$$

Пусть $\lambda = r\phi, \gamma = r$, тогда

$$
 - \frac{2}{r} + r \phi = f, \\
  f = r\phi - \frac{2}{r}
$$